new

LTS.thy
@@ -21,67 +21,172 @@ a path. This leads to the following definition of reachability. Notice,
 that @{term "LTS_is_reachable \<Delta>"} is the reflexive, transitive closure of @{term \<Delta>}.\<close>
 
 
-inductive LTS_is_reachable :: "('q, 'a) LTS   \<Rightarrow>   ('q * 'q) set \<Rightarrow> 'q \<Rightarrow> 'a list \<Rightarrow> 'q \<Rightarrow> bool" where
-   LTS_Empty[intro!]:"LTS_is_reachable l1 l2 q [] q"|
-   LTS_Step1:"(q, q'') \<in> l2 \<and> LTS_is_reachable l1 l2 q'' l q' \<Longrightarrow> LTS_is_reachable l1 l2 q l q'" |
-   LTS_Step2[intro!]:"(\<exists>q'' \<sigma>. a \<in> \<sigma> \<and> (q, \<sigma>, q'') \<in> l1 \<and> LTS_is_reachable l1 l2 q'' w q') \<Longrightarrow> LTS_is_reachable l1 l2 q (a # w) q'"
+inductive LTS_is_reachable :: "(('q, 'a) LTS * ('q * 'q) set) \<Rightarrow> 'q \<Rightarrow> 'a list \<Rightarrow> 'q \<Rightarrow> bool" where
+   LTS_Empty[intro!]:"LTS_is_reachable lts q [] q"|
+   LTS_Step1:"(q, q'') \<in> snd lts \<and> LTS_is_reachable lts q'' l q' \<Longrightarrow> LTS_is_reachable lts q l q'" |
+   LTS_Step2[intro!]:"(\<exists>q'' \<sigma>. a \<in> \<sigma> \<and> (q, \<sigma>, q'') \<in> fst lts \<and> LTS_is_reachable lts q'' w q') \<Longrightarrow> LTS_is_reachable lts q (a # w) q'"
 
 
-lemma subLTSlemma:"LTS_is_reachable l1 l2 q x y \<Longrightarrow> LTS_is_reachable (l1 \<union> l3) (l2 \<union> l4) q x y"
+lemma subLTSlemma:"LTS_is_reachable l1 q x y \<Longrightarrow> LTS_is_reachable (fst l1 \<union> l2, snd l1 \<union> l3) q x y"
   proof (induction rule: LTS_is_reachable.induct)
-    case (LTS_Empty l1 l2 q)
+    case (LTS_Empty lts q)
     then show ?case by auto
   next
-    case (LTS_Step1 q q'' l2 l1 l q')
-    then show ?case apply auto 
-      by (meson LTS_is_reachable.LTS_Step1 UnI1)
+    case (LTS_Step1 q lts l q')
+    then show ?case 
+      by (metis LTS_is_reachable.LTS_Step1 Un_iff snd_conv)
   next
-    case (LTS_Step2 a q l1 l2 w q')
-    then show ?case by auto
+    case (LTS_Step2 a q lts w q')
+    then show ?case 
+      by (smt (z3) LTS_is_reachable.LTS_Step2 UnI1 fst_conv)
   qed
-  
-lemma subLTSlemma1:"LTS_is_reachable l1 l2  q x y \<Longrightarrow> LTS_is_reachable (l1 \<union> {(f q a, va, f q' a)|q va q'. (q,va,q') \<in> l1}) (l2 \<union> l4) q x y"
+
+
+lemma subLTSlemma1:"LTS_is_reachable l1 q x y \<Longrightarrow> LTS_is_reachable (fst l1 \<union> {(f q a, va, f q' a)|q va q'. (q,va,q') \<in> fst l1}, snd l1 \<union> l3) q x y"
   proof (induction rule: LTS_is_reachable.induct)
-    case (LTS_Empty l1 l2 q)
-    then show ?case by auto 
+    case (LTS_Empty lts q)
+    then show ?case by auto
   next
-    case (LTS_Step1 q q'' l2 l1 l q')
-    then show ?case apply auto
+    case (LTS_Step1 q lts l q')
+    then show ?case 
       by (meson LTS_is_reachable.LTS_Step1 subLTSlemma)
   next
-    case (LTS_Step2 a q l1 l2 w q')
-    then show ?case by auto
+    case (LTS_Step2 a q lts w q')
+    then show ?case 
+      by (smt (z3) LTS_is_reachable.LTS_Step2 UnI1 fst_conv)
   qed
 
-lemma DeltLTSlemma1:"LTS_is_reachable l1 l2 q l q' \<Longrightarrow> LTS_is_reachable ({(f q a, va, f q' a)| q va q'. (q, va, q')\<in> l1})  ({(f q a, f q' a)| q q'. (q, q') \<in> l2}) (f q a) l (f q' a)"
-  proof (induction rule: LTS_is_reachable.induct)
-    case (LTS_Empty l1 l2 q)
+lemma DeltLTSlemma1:"LTS_is_reachable lts q l q' \<Longrightarrow>LTS_is_reachable ({(f q a, va, f q' a)| q va q'. (q, va, q')\<in> fst lts}, {(f q a, f q' a)| q q'. (q, q') \<in> snd lts}) (f q a) l (f q' a)"
+  proof (induction rule: LTS_is_reachable.induct)  
+    case (LTS_Empty lts q)
     then show ?case by auto
   next
-    case (LTS_Step1 q q'' l2 l1 l q')
+    case (LTS_Step1 q lts l q')
     then show ?case apply auto
-      by (smt (verit, best) LTS_is_reachable.LTS_Step1 mem_Collect_eq)
+    proof -
+      have "(f q a, f lts a) \<in> snd ({(f aa a, B, f ab a) |aa B ab. (aa, B, ab) \<in> fst l}, {(f aa a, f ab a) |aa ab. (aa, ab) \<in> snd l})"
+        using LTS_Step1.IH by auto
+      then show ?thesis
+        by (smt (z3) LTS_Step1.IH LTS_is_reachable.LTS_Step1)
+    qed
   next
-    case (LTS_Step2 a q l1 l2 w q')
-    then show ?case apply auto 
-      by blast
-  qed  
+    case (LTS_Step2 a q lts w q')
+    then show ?case apply auto by blast
+  qed
 
 
 
 
-lemma joinLTSlemma:"LTS_is_reachable l1 l2 q x p \<Longrightarrow>  LTS_is_reachable l1 l2 p y q''\<Longrightarrow> LTS_is_reachable l1 l2 q (x@y) q''"
+lemma joinLTSlemma:"LTS_is_reachable l q x p \<Longrightarrow>  LTS_is_reachable l p y q''\<Longrightarrow> LTS_is_reachable l q (x@y) q''"
   proof (induction rule: LTS_is_reachable.induct)
-    case (LTS_Empty l1 l2 q)
-    then show ?case by auto
+    case (LTS_Empty lts q)
+    then show ?case apply auto done
   next
-    case (LTS_Step1 q q'' l2 l1 l q')
-    then show ?case apply auto
+    case (LTS_Step1 q lts l q')
+    then show ?case 
       by (meson LTS_is_reachable.LTS_Step1)
   next
-    case (LTS_Step2 a q l1 l2 w q')
-    then show ?case by auto
-  qed 
-
+    case (LTS_Step2 a q lts w q')
+    then show ?case apply auto done
+  qed
 
 end
+
+
+(*
+text \<open> Given a set of states $\mathcal{Q}$ and an alphabet $\Sigma$,
+a labeled transition system is a subset of $\mathcal{Q} \times \Sigma
+\times \mathcal{Q}$.  Given such a relation $\Delta \subseteq
+\mathcal{Q} \times \Sigma \times \mathcal{Q}$, a triple $(q, \sigma,
+q')$ is an element of $\Delta$ iff starting in state $q$ the state
+$q'$ can be reached reading the label $\sigma$. \<close>
+
+  
+type_synonym ('q,'a) LTS = "('q * 'a set * 'q) set"
+
+
+subsubsection  \<open>Reachability\<close>
+
+text \<open>Often it is enough to consider just the first and last state of
+a path. This leads to the following definition of reachability. Notice, 
+that @{term "LTS_is_reachable \<Delta>"} is the reflexive, transitive closure of @{term \<Delta>}.\<close>
+
+inductive LTS_is_reachable :: "('q, 'a) LTS  \<Rightarrow> 'q \<Rightarrow> 'a list \<Rightarrow> 'q \<Rightarrow> bool"  where 
+   LTS_Empty:"LTS_is_reachable \<Delta> q [] q"|
+   LTS_Step:"(\<exists>q'' \<sigma>. a \<in> \<sigma> \<and> (q, \<sigma>, q'') \<in> \<Delta> \<and> LTS_is_reachable \<Delta> q'' w q') \<Longrightarrow> 
+              LTS_is_reachable \<Delta> q (a # w) q'"|
+   LTS_Epi:"(\<exists>q''. (q,{\<epsilon>},q'') \<in> \<Delta> \<and>  LTS_is_reachable \<Delta> q'' [] q') \<Longrightarrow>   LTS_is_reachable \<Delta> q [] q'"|
+   LTS_Epi1:"(\<exists>q''. (q,{\<epsilon>},q'') \<in> \<Delta> \<and>  LTS_is_reachable \<Delta> q'' l q') \<Longrightarrow>   LTS_is_reachable \<Delta> q l q'"
+
+
+inductive_cases LTS_Step_cases[elim!]:"LTS_is_reachable \<Delta> q (a # w) q'"
+
+inductive_cases LTS_Epi_cases[elim!]:"LTS_is_reachable \<Delta> q [] q"
+
+inductive_cases LTS_Epi1_cases[elim!]:"LTS_is_reachable \<Delta> q l q"
+
+
+
+lemma DeltLTSlemma1:"LTS_is_reachable \<Delta> q al y \<Longrightarrow>LTS_is_reachable {(f u, v, f w)| u v w. (u,v,w)\<in> \<Delta> } (f q) al (f y)"
+  proof (induction rule: LTS_is_reachable.induct)
+    case (LTS_Empty \<Delta> q)
+    then show ?case 
+      by (simp add: LTS_is_reachable.LTS_Empty)
+  next
+    case (LTS_Step a q \<Delta> w q')
+    then show ?case 
+      by (smt (verit, best) CollectI LTS_is_reachable.LTS_Step)
+  next
+    case (LTS_Epi q \<Delta> q')
+    then show ?case 
+      by (smt (verit, ccfv_threshold) CollectI LTS_is_reachable.LTS_Epi)
+  next
+    case (LTS_Epi1 q \<Delta> l q')
+    then show ?case 
+      by (metis (mono_tags, lifting) CollectI LTS_is_reachable.LTS_Epi1)
+  qed
+
+lemma subLTSlemma:"LTS_is_reachable l1 q x y \<Longrightarrow> LTS_is_reachable (l1 \<union> l2) q x y"
+  proof (induction rule: LTS_is_reachable.induct)
+    case (LTS_Empty \<Delta> q)
+    then show ?case 
+      by (simp add: LTS_is_reachable.LTS_Empty)
+  next
+    case (LTS_Step a q \<Delta> w q')
+    then show ?case 
+      by (meson LTS_is_reachable.LTS_Step UnI1)
+  next
+    case (LTS_Epi q \<Delta> q')
+    then show ?case 
+      by (meson LTS_is_reachable.LTS_Epi Un_iff)
+  next
+    case (LTS_Epi1 q \<Delta> l q')
+    then show ?case 
+      by (meson LTS_is_reachable.LTS_Epi1 UnI1)
+  qed
+
+
+
+
+lemma joinLTSlemma:"LTS_is_reachable l1 q a y \<Longrightarrow> LTS_is_reachable l1 y b z \<Longrightarrow> LTS_is_reachable l1 q (a@b) z"
+  proof (induction rule: LTS_is_reachable.induct)
+    case (LTS_Empty \<Delta> q)
+    then show ?case 
+      by simp
+  next
+    case (LTS_Step a q \<Delta> w q')
+    then show ?case 
+      by (metis LTS_is_reachable.LTS_Step append_Cons)
+  next
+    case (LTS_Epi q \<Delta> q')
+    then show ?case 
+      by (meson LTS_Epi1)
+  next
+    case (LTS_Epi1 q \<Delta> l q')
+    then show ?case 
+      by (meson LTS_is_reachable.LTS_Epi1)
+  qed
+
+
+
+end*)
