README - 副本.md
@@ -1,2 +1,0 @@
-# REtoNFA
-Conver the regexp into NFA implemented in Isabelle.
